\documentclass{article}

\usepackage[total={7in, 9in}]{geometry}
\usepackage[utf8]{inputenc}
\usepackage[english]{babel}

\usepackage{amsmath}
\usepackage{amssymb}

\usepackage{amsthm}
\newtheorem{lemma}{Lemma}
\theoremstyle{definition}
\newtheorem*{answer}{Answer}

\usepackage{mathtools}
\DeclarePairedDelimiter\ceil{\lceil}{\rceil}
\DeclarePairedDelimiter\floor{\lfloor}{\rfloor}

\newcommand{\evidence}[1]{\ensuremath{\hspace{3em} (\hspace{0.2em} \text{#1} \hspace{0.2em})}}
\newcommand{\asymptotic}[3]{\ensuremath{#2 = #1(#3)}}
\newcommand{\bigO}[2]{\asymptotic{\mathcal{O}}{#1}{#2}}
\newcommand{\bigTheta}[2]{\asymptotic{\Theta}{#1}{#2}}
\newcommand{\relation}[1]{\ensuremath{\hspace{0.2em} {{} #1 {}} \hspace{0.2em}}}
\newcommand{\equal}{\relation{=}}
\newcommand{\lesseq}{\relation{\le}}
\newcommand{\parens}[1]{\left(#1\right)}
\newcommand{\lglg}[1]{\ensuremath{\lg{\parens{\lg{#1}}}}}
\newcommand{\brackets}[1]{\ensuremath{[ \hspace{0.2em} #1 \hspace{0.2em} ]}}
\newcommand{\quantify}[2]{\ensuremath{\forall #1 \in \mathbb{#2}. \hspace{0.2em}}}
\newcommand{\contra}{\ensuremath{\Rightarrow\!\Leftarrow}}

\begin{document}
\noindent
\LARGE\textbf{Math 382: Homework 2} \\
\large Kyle McKean

\section*{Problem 1}

\begin{lemma}
  \begin{equation*}
    \phi(n) := R(n) \le 2n
  \end{equation*}
\end{lemma}
\begin{proof}
  \hfill
  \begin{itemize}
  \item
    \textit{Base Case}: $\phi(1)$
    \begin{align*}
      R(1) &\le 2 \times 1 \\
      1    &\le 2
    \end{align*}
  \item
    \textit{Inductive Step}: assume $\phi(k)$ for all $k \le n$ to prove $\phi(n + 1)$
    \begin{alignat*}{4}
      & R(n + 1) & \equal  & R\parens{\floor*{\frac{n + 1}{2}}} + (n + 1) & \evidence{Definition of $R$} \\
      & {}       & \lesseq & 2\floor*{\frac{n + 1}{2}} + n + 1            & \evidence{Inductive Hypothesis} \\
      & {}       & \equal  & n + 1 + n + 1                                & {} \\
      & {}       & \equal  & 2 (n + 1)                                    & \qedhere
    \end{alignat*}
  \end{itemize}
\end{proof}
\begin{answer}[A]
  Lemma 1 tells us $\bigO{R(n)}{n}$ where $m = 1$ and $c = 2$
\end{answer}

\begin{lemma}
  \begin{equation*}
    \phi(n) := Q(n) \le 2\lglg{n}
  \end{equation*}
\end{lemma}
\begin{proof}
  \hfill
  \begin{itemize}
  \item
    \textit{Base Case}: $\phi(4)$
    \begin{align*}
      Q(4) &\le 2\lglg{4} \\
      2 &\le 2
    \end{align*}
  \item
    \textit{Inductive Step}: assume $\phi(k)$ for all $k \le n$ to prove $\phi(n + 1)$
    \begin{alignat*}{4}
      & Q(n + 1) & \equal & Q\left(\floor*{\sqrt{n + 1}}\right) + 1 & \evidence{Definition of $Q$} \\
      & {}       & \lesseq & 2\lglg{\floor*{\sqrt{n + 1}}} + 1       & \evidence{Inductive Hypothesis} \\
      & {}       & \lesseq & 2\lglg{\sqrt{n + 1}} + 1                & \evidence{$\forall x. \hspace{0.2em} \floor*{x} \le x$} \\
      & {}       & \equal  & 2\lg{\parens{\frac{1}{2}\lg{\parens{n + 1}}}} + 1     & {} \\
      & {}       & \equal  & 2\parens{\lg{1} - \lg{2} + \lglg{\parens{n + 1}}} + 1 & {} \\
      & {}       & \equal  & {-2} + 2\lglg{\parens{n + 1}} + 1                     & {} \\
      & {}       & \equal  & 2\lglg{\parens{n + 1}} - 1                            & {} \\
      & {}       & \lesseq & 2\lglg{\parens{n + 1}}                                & \qedhere
    \end{alignat*}
  \end{itemize}
\end{proof}
\begin{answer}[B]
  Lemma 2 tells us $\bigO{Q(n)}{\lglg{n}}$ where $m = 4$ and $c = 2$
\end{answer}

\section*{Problem 2}

\begin{lemma}
  \begin{equation*}
    \quantify{n, i}{N} 4 \le n \wedge i \le n \Rightarrow n \le (n - i + 1)
  \end{equation*} 
\end{lemma} 

\begin{proof}
  Verified with the Z3 STM solver \qedhere
\end{proof}

\begin{lemma}
  \begin{equation*}
    \quantify{n}{N} 1 \le n \Rightarrow \lg{\parens{n!}} \le n \lg{n}
  \end{equation*} 
\end{lemma}
\noindent
To solve the above proposition we observe the equation expands to pairwise less than or equals.
\begin{equation*}
  \lg{1} + \lg{2} + \dots + \lg{n} \le \lg{n} + \lg{n} + \dots + \lg{n}
\end{equation*} 
\begin{proof}
      
  \begin{alignat*}{4}
    & \lg{n!} & \equal  & \lg{\prod_{i=1}^{n}{i}}  & \evidence{definition of factorial} \\
    & {}      & \equal  & \sum_{i=1}^{n}{\lg{i}}   & \evidence{log product rule} \\
    & {}      & \lesseq & \sum_{i=1}^{n}{\lg{n}}   & \evidence{$i \le n$} \\  
    & {}      & \equal  & n \lg{n}                & \qedhere
  \end{alignat*}
\end{proof}

\begin{lemma}
  \begin{equation*}
    \quantify{n}{N} 4 \le n \Rightarrow \frac{n}{2} \lg{n} \le \lg{\parens{n!}}
  \end{equation*} 
\end{lemma} 
\noindent
To solve the next proposition we rearrange the term right of the relation.
Then we observe two of the terms on the right add to more than one on the left.
The following is an example when $n = 6$.
\begin{equation*}
  \brackets{\lg{6}} + \brackets{\lg{6}} + \brackets{\lg{6}} \le
  \brackets{\lg{1} + \lg{6}} + \brackets{\lg{2} + \lg{5}} + \brackets{\lg{3} + \lg{4}}
\end{equation*}

\begin{proof}
  \hfill
  \begin{itemize}
    \item n is even
      \begin{alignat*}{4}
        & \frac{n}{2}\lg{n} & \equal  & \sum_{i=1}^{n/2}{\lg{n}}            & \evidence{definition of factorial} \\
        & {}                & \lesseq & \sum_{i=1}^{n/2}{\lg{i(n - i + 1)}} & \evidence{lemma 3} \\
        & {}                & \equal  & \sum_{i=1}^{n/2}{\lg{i} + \lg{(n - i + 1)}} & {} \\
        & {}                & \equal  & \sum_{i=1}^{n/2}{\lg{i}} + \sum_{i=1}^{n/2}{\lg{(n - i + 1)}} & {} \\
        & {}                & \equal  & \sum_{i=1}^{n/2}{\lg{i}} + \sum_{i=n/2 + 1}^{n}{\lg{i}} & \evidence{readjust bounds} \\
        & {}                & \equal  & \sum_{i=1}^{n}{\lg{i}}   & {} \\
        & {}                & \equal  & \lg{\prod_{i=1}^{n}{i}}  & \evidence{log product rule} \\
        & {}                & \equal  & \lg{n!}                   & {}
      \end{alignat*}
    \item n is odd
  \end{itemize}
\end{proof}

\begin{answer}
  \hfill
  \begin{proof}
    \vspace{1em}
    \begin{equation*}
      0 \le \frac{1}{2} \times n \lg{n} \le \lg{n!} \le 1 \times n\lg{n} \evidence{By Lemma 4 $\&$ 5}
    \end{equation*}
    So $\bigTheta{\lg{n!}}{n\lg{n}}$ where $c_1 = \frac{1}{2}$, $c_2 = 1$, and $m = 4$ $\qedhere$ 
  \end{proof}
\end{answer}

\section*{Problem 3}

\section*{Problem 4}

\begin{lemma}
  \begin{equation*}
    \quantify{a, b}{R} 1 \le a \wedge 1 \le b \Rightarrow a + b \le 2ab
  \end{equation*}
\end{lemma}

\begin{proof}
  Verified with the Z3 STM solver and its unstable support for Real Analysis \qedhere
\end{proof}


\begin{answer}[A]
  \hfill
  \begin{proof}
    $\quantify{n}{N} m \le n$ where m is the lowest q required to satsify $\bigO{f(q)}{g(q)}$
    \begin{alignat*}{4}
      & 0  & \lesseq & \lg{f(n)}                   & {} \\
      & {} & \lesseq & \lg{\parens{c \times g(n)}} & \evidence{$f(n) \le  c \times g(n)$ for some $c$ } \\
      & {} & \equal  & \lg{c} + \lg{\parens{g(n)}} & {} \\
      & {} & \equal  & (2\lg{c} \times \lg{g(n)}   & \evidence{By the above lemma where $a = \lg{c}$ and $b = \lg{\parens{g(n)}}$}
  \end{alignat*}
  So $\bigO{\lg{f(n)}}{\lg{g(n)}}$ where $c_1 = 2\lg{c}$ and $m_1 = m$ \qedhere
  \end{proof}
  
\end{answer}

\begin{answer}[B]
  $\bigO{2n^2}{n^2}$ trivally true so assume $\bigO{2^{2n^2}}{2^{n^2}}$
  \begin{alignat*}{4}
      & 2^{2n^2}             & \lesseq & c \times 2^{n^2}                    & {} \\
      & {\parens{2^{n^2}}}^2 & \lesseq & c \times 2^{n^2}                    & \evidence{Divide by $2^{n^2}$} \\
      & 2^{n^2}              & \lesseq & c                                  & {}
  \end{alignat*}
  We now see our assumption is incorrect because:
  $\nexists c \in \mathbb{R}. \hspace{0.2em} \quantify{n}{N} 2^{n^2} \le c \hfill \contra$
\end{answer}

\begin{answer}[C]
  
  \hfill
  \begin{proof}
    $\quantify{n}{N} m \le n$ where m is the lowest q required to satsify $\bigO{f(q)}{g(q)}$
    \begin{alignat*}{4}
      & 0  & \lesseq & 1 \times f(n)          & {} \\
      & {} & \lesseq & f(n) + g(n)   & \evidence{$0 \le g(n)$} \\
      & {} & \lesseq & 2 \times f(n) & \evidence{$g(n) \le f(n)$}
  \end{alignat*}
  So $\bigTheta{f(n)}{g(n)}$ where $c_1 = 1$, $c_2 = 2$ and $m_1 = m$ \qedhere
  \end{proof}
\end{answer}

\section*{Problem 5}

\end{document}

